Revamp LinearSequence.i.dfy to present A not maybe<A>

examples/LinearSequence.i.dfy
@@ -3,11 +3,16 @@ include "../lib/Base/sequences.i.dfy"
 include "LinearMaybe.s.dfy"
 include "LinearSequence.s.dfy"
 
-import opened Sequences
-
-// module LinearSequence_i {
-  // import opened LinearMaybe
-  // import opened LinearSequence
+module LinearSequence_i {
+  import opened LinearMaybe
+  import opened LinearSequence_s
+  import opened Sequences
+  export
+    provides LinearSequence_s
+    provides seq_alloc_init, lseqs, lseq_has, lseq_length, lseq_peek
+    provides lseq_alloc, lseq_free, lseq_swap, lseq_take, lseq_give
+    reveals lseq_full
+    reveals operator'cardinality?lseq, operator'in?lseq, operator'subscript?lseq
 
   method seq_alloc_init<A>(length:nat, a:A) returns(linear s:seq<A>)
       ensures |s| == length
@@ -25,51 +30,96 @@ import opened Sequences
       }
   }
 
-  function{:inline true} operator(| |)<A>(s:lseq<A>):nat
+  function lseqs<A>(l:lseq<A>):(s:seq<A>)
   {
-      |lseqs(s)|
+      Apply(read, lseqs_raw(l))
   }
 
-  function{:inline true} operator([])<A>(s:lseq<A>, i:nat):A
-      requires i < |s|
+  function lseq_has<A>(l:lseq<A>):(s:seq<bool>)
+      ensures |s| == |lseqs(l)|
   {
-      read(lseqs(s)[i])
+      Apply(has, lseqs_raw(l))
+  }
+
+  function method lseq_length<A>(shared s:lseq<A>):(n:nat)
+      ensures n == |lseqs(s)|
+  {
+      lseq_length_raw(s)
+  }
+
+  function method lseq_peek<A>(shared s:lseq<A>, i:nat):(shared a:A)
+      requires i < |lseqs(s)|
+      requires lseq_has(s)[i]
+      ensures a == lseqs(s)[i]
+  {
+      peek(lseq_share_raw(s, i))
+  }
+
+  function method{:inline true} operator(| |)<A>(shared s:lseq<A>):nat
+  {
+      lseq_length(s)
   }
 
   function{:inline true} operator(in)<A>(s:lseq<A>, i:nat):bool
       requires i < |s|
   {
-      has(lseqs(s)[i])
+      lseq_has(s)[i]
   }
 
-  function method lseq_peek<A>(shared s:lseq<A>, i:nat):(shared a:A)
+  function{:inline true} operator([])<A>(s:lseq<A>, i:nat):A
       requires i < |s|
-      requires i in s
-      ensures a == s[i]
   {
-      peek(lseq_share(s, i))
+      lseqs(s)[i]
+  }
+
+  method lseq_alloc<A>(length:nat) returns(linear s:lseq<A>)
+      ensures |s| == length
+      ensures forall i:nat | i < length :: i !in s
+  {
+      s := lseq_alloc_raw(length);
+  }
+
+  method lseq_free<A>(linear s:lseq<A>)
+      requires forall i:nat | i < |s| :: i !in s
+  {
+      assert forall i:nat {:trigger lseqs_raw(s)[i]} | i < |lseqs_raw(s)| :: i !in s;
+      lseq_free_raw(s);
+  }
+
+  // can be implemented as in-place swap
+  method lseq_swap<A>(linear s1:lseq<A>, i:nat, linear a1:A) returns(linear s2:lseq<A>, linear a2:A)
+      requires i < |s1| && i in s1
+      ensures a2 == s1[i]
+      ensures lseq_has(s2) == lseq_has(s1)
+      ensures lseqs(s2) == lseqs(s1)[i := a1]
+  {
+      linear var x1:maybe<A> := give(a1);
+      linear var x2:maybe<A>;
+      s2, x2 := lseq_swap_raw(s1, i, x1);
+      a2 := unwrap(x2);
   }
 
   method lseq_take<A>(linear s1:lseq<A>, i:nat) returns(linear s2:lseq<A>, linear a:A)
-      requires i < |s1|
-      requires i in s1
+      requires i < |s1| && i in s1
       ensures a == s1[i]
-      ensures lseqs(s2) == lseqs(s1)[i := empty()]
+      ensures lseq_has(s2) == lseq_has(s1)[i := false]
+      ensures forall j:nat | j < |s1| && j != i :: lseqs(s2)[j] == lseqs(s1)[j]
   {
       linear var x1:maybe<A> := empty();
       linear var x2:maybe<A>;
-      s2, x2 := lseq_swap(s1, i, x1);
+      s2, x2 := lseq_swap_raw(s1, i, x1);
       a := unwrap(x2);
   }
 
   method lseq_give<A>(linear s1:lseq<A>, i:nat, linear a:A) returns(linear s2:lseq<A>)
       requires i < |s1|
-      requires !(i in s1)
-      ensures lseqs(s2) == lseqs(s1)[i := give(a)]
+      requires i !in s1
+      ensures lseq_has(s2) == lseq_has(s1)[i := true]
+      ensures lseqs(s2) == lseqs(s1)[i := a]
   {
       linear var x1:maybe<A> := give(a);
       linear var x2:maybe<A>;
-      s2, x2 := lseq_swap(s1, i, x1);
+      s2, x2 := lseq_swap_raw(s1, i, x1);
       var _ := discard(x2);
   }
 
@@ -77,13 +127,20 @@ import opened Sequences
   {
       && (forall i | 0 <= i < |s| :: i in s)
   }
+} // module
 
-  function{:opaque} lseqs_full<A>(s: lseq<A>): (result: seq<A>)
-      requires lseq_full(s)
-      ensures |result| == |s|
-      ensures forall i | 0 <= i < |s| :: result[i] == s[i]
+module Test
+{
+  import opened LinearMaybe
+  import opened LinearSequence_s
+  import opened LinearSequence_i
+  method T(linear l:lseq<int>)
+      requires |l| > 0
+      requires forall i:nat | i < |l| :: i !in l
   {
-      Apply(x requires has(x) => peek(x), lseqs(s))
+      assert 0 !in l;
+      assert !lseq_has(l)[0];
+      // should fail: assert !has(lseqs_raw(l)[0]);
+      lseq_free(l);
   }
-
-// } // module
+}
